src/smtencoding/FStarC.SMTEncoding.Pruning.fsti
@@ -14,7 +14,6 @@
    limitations under the License.
 *)
 module FStarC.SMTEncoding.Pruning
-#push-options "--MLish --MLish_effect FStarC.Effect"
 (**
   This module provides support for the '--ext context_pruning' feature.
 
@@ -56,7 +55,7 @@ val pruning_state  : Type0
 val init : pruning_state
 
 (* Adding assumptions to the pruning state *)
-val add_decls (ds:list decl) (p:pruning_state) : pruning_state
+val add_decls (ds:list decl) (p:pruning_state) : ML pruning_state
 
 (* Pruning the state to only include the assumptions that are reachable from the roots *)
-val prune (p:pruning_state) (roots:list decl) : list decl
+val prune (p:pruning_state) (roots:list decl) : ML (list decl)
